# Socks shoe property

Let $G$ be a group. If $a, b \in G$, then $(ab)^{-1} = b^{-1}a^{-1}$

## Proof

Since $(ab)(ab)^{-1} = e$ and $(ab)(b^{-1}a^{-1}) = a(b b^{-1})a^{-1} = a e a^{-1} = a a^{-1} = e$, we have by [**uniqueness of an inverse element**](./0005-inverse-of-element-in-a-group-is-unique.md) that $(ab)^{-1} = b^{-1}a^{-1}$.

## Reference

1. Joseph A. Gallian, *Contemporary Abstract Algebra* (page 50)
2. [abstract.pugetsound.edu Proposition 3.19](https://abstract.ups.edu/abstract.ups.edu/aata/groups-section-defnitions.html)